Rocq/src/TypedExprPath.v
@@ -15,69 +15,69 @@ Module TypedExprPath.
   | TP_Empty : forall e,
       IsTypedPath e []
   | TP_LhsBinOp : forall s lhs rhs p,
-      IsTypedPath lhs p -> IsTypedPath (TBinOp s lhs rhs) (Left :: p)
+      IsTypedPath lhs p -> IsTypedPath (TBinOp s lhs rhs) (0 :: p)
   | TP_RhsBinOp : forall s lhs rhs p,
-      IsTypedPath rhs p -> IsTypedPath (TBinOp s lhs rhs) (Right :: p)
+      IsTypedPath rhs p -> IsTypedPath (TBinOp s lhs rhs) (1 :: p)
   | TP_UnOpArg : forall s arg p,
-      IsTypedPath arg p -> IsTypedPath (TUnOp s arg) (Arg :: p)
+      IsTypedPath arg p -> IsTypedPath (TUnOp s arg) (0 :: p)
   | TP_CastArg : forall s arg p,
-      IsTypedPath arg p -> IsTypedPath (TCast s arg) (Arg :: p)
+      IsTypedPath arg p -> IsTypedPath (TCast s arg) (0 :: p)
   | TP_LhsCompOp : forall s lhs rhs p,
-      IsTypedPath lhs p -> IsTypedPath (TComp s lhs rhs) (Left :: p)
+      IsTypedPath lhs p -> IsTypedPath (TComp s lhs rhs) (0 :: p)
   | TP_RhsCompOp : forall s lhs rhs p,
-      IsTypedPath rhs p -> IsTypedPath (TComp s lhs rhs) (Right :: p)
+      IsTypedPath rhs p -> IsTypedPath (TComp s lhs rhs) (1 :: p)
   | TP_LhsLogic : forall s lhs rhs p,
-      IsTypedPath lhs p -> IsTypedPath (TLogic s lhs rhs) (Left :: p)
+      IsTypedPath lhs p -> IsTypedPath (TLogic s lhs rhs) (0 :: p)
   | TP_RhsLogic : forall s lhs rhs p,
-      IsTypedPath rhs p -> IsTypedPath (TLogic s lhs rhs) (Right :: p)
+      IsTypedPath rhs p -> IsTypedPath (TLogic s lhs rhs) (1 :: p)
   | TP_RedArg : forall s arg p,
-      IsTypedPath arg p -> IsTypedPath (TReduction s arg) (Arg :: p)
+      IsTypedPath arg p -> IsTypedPath (TReduction s arg) (0 :: p)
   | TP_LhsShift : forall s lhs rhs p,
-      IsTypedPath lhs p -> IsTypedPath (TShift s lhs rhs) (Left :: p)
+      IsTypedPath lhs p -> IsTypedPath (TShift s lhs rhs) (0 :: p)
   | TP_RhsShift : forall s lhs rhs p,
-      IsTypedPath rhs p -> IsTypedPath (TShift s lhs rhs) (Right :: p)
+      IsTypedPath rhs p -> IsTypedPath (TShift s lhs rhs) (1 :: p)
   | TP_AssignArg : forall s op arg p,
-      IsTypedPath arg p -> IsTypedPath (TAssign s op arg) (Arg :: p)
+      IsTypedPath arg p -> IsTypedPath (TAssign s op arg) (0 :: p)
   | TP_ShiftAssignArg : forall s op arg p,
-      IsTypedPath arg p -> IsTypedPath (TShiftAssign s op arg) (Arg :: p)
+      IsTypedPath arg p -> IsTypedPath (TShiftAssign s op arg) (0 :: p)
   | TP_CondCond : forall s cond tb fb p,
-      IsTypedPath cond p -> IsTypedPath (TCond s cond tb fb) (Arg :: p)
+      IsTypedPath cond p -> IsTypedPath (TCond s cond tb fb) (0 :: p)
   | TP_CondTrue : forall s cond tb fb p,
-      IsTypedPath tb p -> IsTypedPath (TCond s cond tb fb) (Left :: p)
+      IsTypedPath tb p -> IsTypedPath (TCond s cond tb fb) (1 :: p)
   | TP_CondFalse : forall s cond tb fb p,
-      IsTypedPath fb p -> IsTypedPath (TCond s cond tb fb) (Right :: p)
+      IsTypedPath fb p -> IsTypedPath (TCond s cond tb fb) (2 :: p)
   | TP_ConcatArgs : forall s n args e p,
       nth_error args n = Some e -> IsTypedPath e p ->
-      IsTypedPath (TConcat s args) (Args n :: p)
+      IsTypedPath (TConcat s args) (n :: p)
   | TP_ReplArg : forall s i arg p,
-      IsTypedPath arg p -> IsTypedPath (TRepl s i arg) (Arg :: p)
+      IsTypedPath arg p -> IsTypedPath (TRepl s i arg) (0 :: p)
   .
 
   Fixpoint sub_typed_expr (e: TypedExpr) (p: path) :=
     match e, p with
     | e, [] => Some e
-    | TBinOp _ lhs _, Left :: p => sub_typed_expr lhs p
-    | TBinOp _ _ rhs, Right :: p => sub_typed_expr rhs p
-    | TUnOp _ arg, Arg :: p => sub_typed_expr arg p
-    | TCast _ arg, Arg :: p => sub_typed_expr arg p
-    | TComp _ lhs _, Left :: p => sub_typed_expr lhs p
-    | TComp _ _ rhs, Right :: p => sub_typed_expr rhs p
-    | TLogic _ lhs _, Left :: p => sub_typed_expr lhs p
-    | TLogic _ _ rhs, Right :: p => sub_typed_expr rhs p
-    | TReduction _ arg, Arg :: p => sub_typed_expr arg p
-    | TShift _ lhs _, Left :: p => sub_typed_expr lhs p
-    | TShift _ _ rhs, Right :: p => sub_typed_expr rhs p
-    | TAssign _ _ arg, Arg :: p => sub_typed_expr arg p
-    | TShiftAssign _ _ arg, Arg :: p => sub_typed_expr arg p
-    | TCond _ cond _ _, Arg :: p => sub_typed_expr cond p
-    | TCond _ _ tb _, Left :: p => sub_typed_expr tb p
-    | TCond _ _ _ fb, Right :: p => sub_typed_expr fb p
-    | TConcat _ args, Args i :: p =>
+    | TBinOp _ lhs _, 0:: p => sub_typed_expr lhs p
+    | TBinOp _ _ rhs, 1 :: p => sub_typed_expr rhs p
+    | TUnOp _ arg, 0 :: p => sub_typed_expr arg p
+    | TCast _ arg, 0 :: p => sub_typed_expr arg p
+    | TComp _ lhs _, 0 :: p => sub_typed_expr lhs p
+    | TComp _ _ rhs, 1 :: p => sub_typed_expr rhs p
+    | TLogic _ lhs _, 0 :: p => sub_typed_expr lhs p
+    | TLogic _ _ rhs, 1 :: p => sub_typed_expr rhs p
+    | TReduction _ arg, 0 :: p => sub_typed_expr arg p
+    | TShift _ lhs _, 0 :: p => sub_typed_expr lhs p
+    | TShift _ _ rhs, 1 :: p => sub_typed_expr rhs p
+    | TAssign _ _ arg, 0 :: p => sub_typed_expr arg p
+    | TShiftAssign _ _ arg, 0 :: p => sub_typed_expr arg p
+    | TCond _ cond _ _, 0 :: p => sub_typed_expr cond p
+    | TCond _ _ tb _, 1 :: p => sub_typed_expr tb p
+    | TCond _ _ _ fb, 2 :: p => sub_typed_expr fb p
+    | TConcat _ args, i :: p =>
         match nth_error args i with
         | Some e => sub_typed_expr e p
         | None => None
         end
-    | TRepl _ _ arg, Arg :: p => sub_typed_expr arg p
+    | TRepl _ _ arg, 0 :: p => sub_typed_expr arg p
     | _, _ :: _ => None
     end
   .
@@ -94,21 +94,24 @@ Module TypedExprPath.
   Lemma sub_typed_expr_valid: forall e p f, e @@[p] = Some f -> IsTypedPath e p.
   Proof.
     induction e using TypedExpr_ind; intros;
-      try (destruct p as [|[]]; try (discriminate H); constructor; firstorder).
-      - destruct p as [|[]]; try (discriminate H); try (discriminate H0).
-        + constructor.
-        + simpl in H0. destruct (nth_error args i) eqn:H1; try (discriminate H0).
-          econstructor. eassumption. apply (H _ _ H1 _ _ H0).
+      try (destruct p as [|[|[|[]]]]; simpl in *;
+           (constructor; firstorder) || congruence).
+    - destruct p.
+      + constructor.
+      + destruct (nth_error args n) eqn:H1; simpl in H0; rewrite H1 in H0.
+        * apply (TP_ConcatArgs _ _ _ _ _ H1 (H _ _ H1 _ _ H0)).
+        * congruence.
   Qed.
 
-  Lemma IsTypedPath_sub_typed_expr_iff: forall e p, IsTypedPath e p <-> exists e0, e @@[p] = Some e0.
+  Lemma IsTypedPath_sub_typed_expr_iff:
+    forall e p, IsTypedPath e p <-> exists e0, e @@[p] = Some e0.
   Proof.
     split.
     - apply IsTypedPath_is_sub_typed_expr.
     - intros [? H]. apply (sub_typed_expr_valid _ _ _ H).
   Qed.
 
-  Lemma sub_typed_expr_nil: forall e, e @@[ [] ] = Some e.
+  Lemma sub_typed_expr_nil: forall e, e @@[[]] = Some e.
   Proof.
     intros. destruct e; reflexivity.
   Qed.
@@ -119,13 +122,12 @@ Module TypedExprPath.
     induction p; split; intros.
     - destruct H as [f [H1 H2]]. rewrite sub_typed_expr_nil in H1. inv H1. assumption.
     - exists e. split. apply sub_typed_expr_nil. assumption.
-    - destruct H as [f [H1 H2]]. destruct e; simpl; try (discriminate H1);
-        destruct a; simpl in *; try (destruct (nth_error _ i));
-        (apply IHp; exists f; intuition) || discriminate H1.
-    - destruct a; simpl in H;
-        try (destruct e; discriminate H || (apply IHp in H; assumption));
-        destruct e; discriminate H || (destruct (nth_error _ i) eqn:H';
-        discriminate H || (apply IHp in H; simpl; rewrite H'; assumption)).
+    - destruct H as [f [H1 H2]]. destruct e; simpl in *;
+        try congruence; try (destruct (nth_error _ a)); destruct a as [|[|[]]];
+        congruence || (apply IHp; eexists; intuition; eassumption).
+    - destruct e; simpl in *;
+        try congruence; try (destruct (nth_error _ a));
+        destruct a as [|[|[]]]; congruence || apply IHp; assumption.
   Qed.
 
   Lemma IsTypedPath_chunk : forall e p c,
@@ -133,8 +135,9 @@ Module TypedExprPath.
   Proof.
     split; intros.
     - destruct (IsTypedPath_is_sub_typed_expr _ _ H) as [g H1].
-      apply sub_typed_expr_chunk in H1. destruct H1 as [f [H2 H3]].
-      exists f. split. assumption. apply IsTypedPath_sub_typed_expr_iff.
+      apply sub_typed_expr_chunk in H1.
+      destruct H1 as [f [H2 H3]]. exists f. split. assumption.
+      apply IsTypedPath_sub_typed_expr_iff.
       exists g. assumption.
     - destruct H as [f [H1 H2]]. apply IsTypedPath_sub_typed_expr_iff.
       apply IsTypedPath_sub_typed_expr_iff in H2. destruct H2 as [g H2]. exists g.
