Rocq/src/ExprPath.v
@@ -15,68 +15,68 @@ Module ExprPath.
   | P_Empty : forall e,
       IsPath e []
   | P_LhsBinOp : forall lhs rhs p,
-      IsPath lhs p -> IsPath (EBinOp lhs rhs) (Left :: p)
+      IsPath lhs p -> IsPath (EBinOp lhs rhs) (0 :: p)
   | P_RhsBinOp : forall lhs rhs p,
-      IsPath rhs p -> IsPath (EBinOp lhs rhs) (Right :: p)
+      IsPath rhs p -> IsPath (EBinOp lhs rhs) (1 :: p)
   | P_UnOpArg : forall arg p,
-      IsPath arg p -> IsPath (EUnOp arg) (Arg :: p)
+      IsPath arg p -> IsPath (EUnOp arg) (0 :: p)
   | P_CastArg : forall arg p,
-      IsPath arg p -> IsPath (ECast arg) (Arg :: p)
+      IsPath arg p -> IsPath (ECast arg) (0 :: p)
   | P_LhsCompOp : forall lhs rhs p,
-      IsPath lhs p -> IsPath (EComp lhs rhs) (Left :: p)
+      IsPath lhs p -> IsPath (EComp lhs rhs) (0 :: p)
   | P_RhsCompOp : forall lhs rhs p,
-      IsPath rhs p -> IsPath (EComp lhs rhs) (Right :: p)
+      IsPath rhs p -> IsPath (EComp lhs rhs) (1 :: p)
   | P_LhsLogic : forall lhs rhs p,
-      IsPath lhs p -> IsPath (ELogic lhs rhs) (Left :: p)
+      IsPath lhs p -> IsPath (ELogic lhs rhs) (0 :: p)
   | P_RhsLogic : forall lhs rhs p,
-      IsPath rhs p -> IsPath (ELogic lhs rhs) (Right :: p)
+      IsPath rhs p -> IsPath (ELogic lhs rhs) (1 :: p)
   | P_RedArg : forall arg p,
-      IsPath arg p -> IsPath (EReduction arg) (Arg :: p)
+      IsPath arg p -> IsPath (EReduction arg) (0 :: p)
   | P_LhsShift : forall lhs rhs p,
-      IsPath lhs p -> IsPath (EShift lhs rhs) (Left :: p)
+      IsPath lhs p -> IsPath (EShift lhs rhs) (0 :: p)
   | P_RhsShift : forall lhs rhs p,
-      IsPath rhs p -> IsPath (EShift lhs rhs) (Right :: p)
+      IsPath rhs p -> IsPath (EShift lhs rhs) (1 :: p)
   | P_AssignArg : forall op arg p,
-      IsPath arg p -> IsPath (EAssign op arg) (Arg :: p)
+      IsPath arg p -> IsPath (EAssign op arg) (0 :: p)
   | P_ShiftAssignArg : forall op arg p,
-      IsPath arg p -> IsPath (EShiftAssign op arg) (Arg :: p)
+      IsPath arg p -> IsPath (EShiftAssign op arg) (0 :: p)
   | P_CondCond : forall cond tb fb p,
-      IsPath cond p -> IsPath (ECond cond tb fb) (Arg :: p)
+      IsPath cond p -> IsPath (ECond cond tb fb) (0 :: p)
   | P_CondTrue : forall cond tb fb p,
-      IsPath tb p -> IsPath (ECond cond tb fb) (Left :: p)
+      IsPath tb p -> IsPath (ECond cond tb fb) (1 :: p)
   | P_CondFalse : forall cond tb fb p,
-      IsPath fb p -> IsPath (ECond cond tb fb) (Right :: p)
+      IsPath fb p -> IsPath (ECond cond tb fb) (2 :: p)
   | P_ConcatArgs : forall n args e p,
-      nth_error args n = Some e -> IsPath e p -> IsPath (EConcat args) (Args n :: p)
+      nth_error args n = Some e -> IsPath e p -> IsPath (EConcat args) (n :: p)
   | P_ReplArg : forall i arg p,
-      IsPath arg p -> IsPath (ERepl i arg) (Arg :: p)
+      IsPath arg p -> IsPath (ERepl i arg) (0 :: p)
   .
 
   Fixpoint sub_expr (e: Expr) (p: path) :=
     match e, p with
     | e, [] => Some e
-    | EBinOp lhs _, Left :: p => sub_expr lhs p
-    | EBinOp _ rhs, Right :: p => sub_expr rhs p
-    | EUnOp arg, Arg :: p => sub_expr arg p
-    | ECast arg, Arg :: p => sub_expr arg p
-    | EComp lhs _, Left :: p => sub_expr lhs p
-    | EComp _ rhs, Right :: p => sub_expr rhs p
-    | ELogic lhs _, Left :: p => sub_expr lhs p
-    | ELogic _ rhs, Right :: p => sub_expr rhs p
-    | EReduction arg, Arg :: p => sub_expr arg p
-    | EShift lhs _, Left :: p => sub_expr lhs p
-    | EShift _ rhs, Right :: p => sub_expr rhs p
-    | EAssign _ arg, Arg :: p => sub_expr arg p
-    | EShiftAssign _ arg, Arg :: p => sub_expr arg p
-    | ECond cond _ _, Arg :: p => sub_expr cond p
-    | ECond _ tb _, Left :: p => sub_expr tb p
-    | ECond _ _ fb, Right :: p => sub_expr fb p
-    | EConcat args, Args i :: p =>
+    | EBinOp lhs _, 0 :: p => sub_expr lhs p
+    | EBinOp _ rhs, 1 :: p => sub_expr rhs p
+    | EUnOp arg, 0 :: p => sub_expr arg p
+    | ECast arg, 0 :: p => sub_expr arg p
+    | EComp lhs _, 0 :: p => sub_expr lhs p
+    | EComp _ rhs, 1 :: p => sub_expr rhs p
+    | ELogic lhs _, 0 :: p => sub_expr lhs p
+    | ELogic _ rhs, 1 :: p => sub_expr rhs p
+    | EReduction arg, 0 :: p => sub_expr arg p
+    | EShift lhs _, 0 :: p => sub_expr lhs p
+    | EShift _ rhs, 1 :: p => sub_expr rhs p
+    | EAssign _ arg, 0 :: p => sub_expr arg p
+    | EShiftAssign _ arg, 0 :: p => sub_expr arg p
+    | ECond cond _ _, 0 :: p => sub_expr cond p
+    | ECond _ tb _, 1 :: p => sub_expr tb p
+    | ECond _ _ fb, 2 :: p => sub_expr fb p
+    | EConcat args, i :: p =>
         match nth_error args i with
         | Some e => sub_expr e p
         | None => None
         end
-    | ERepl _ arg, Arg :: p => sub_expr arg p
+    | ERepl _ arg, 0 :: p => sub_expr arg p
     | _, _ :: _ => None
     end
   .
@@ -93,11 +93,13 @@ Module ExprPath.
   Lemma sub_expr_valid: forall e p f, e @[p] = Some f -> IsPath e p.
   Proof.
     induction e using Expr_ind; intros;
-      try (destruct p as [|[]]; try (discriminate H); constructor; firstorder).
-      - destruct p as [|[]]; try (discriminate H); try (discriminate H0).
-        + constructor.
-        + simpl in H0. destruct (nth_error args i) eqn:H1; try (discriminate H0).
-          econstructor. eassumption. apply (H _ _ H1 _ _ H0).
+      try (destruct p as [|[|[|[]]]]; simpl in *;
+           (constructor; firstorder) || congruence).
+    - destruct p.
+      + constructor.
+      + destruct (nth_error args n) eqn:H1; simpl in H0; rewrite H1 in H0.
+        * apply (P_ConcatArgs _ _ _ _ H1 (H _ _ H1 _ _ H0)).
+        * congruence.
   Qed.
 
   Lemma IsPath_sub_expr_iff: forall e p, IsPath e p <-> exists e0, e @[p] = Some e0.
@@ -118,13 +120,12 @@ Module ExprPath.
     induction p; split; intros.
     - destruct H as [f [H1 H2]]. rewrite sub_expr_nil in H1. inv H1. assumption.
     - exists e. split. apply sub_expr_nil. assumption.
-    - destruct H as [f [H1 H2]]. destruct e; simpl; try (discriminate H1);
-        destruct a; simpl in *; try (destruct (nth_error _ i));
-        (apply IHp; exists f; intuition) || discriminate H1.
-    - destruct a; simpl in H;
-        try (destruct e; discriminate H || (apply IHp in H; assumption));
-        destruct e; discriminate H || (destruct (nth_error _ i) eqn:H';
-        discriminate H || (apply IHp in H; simpl; rewrite H'; assumption)).
+    - destruct H as [f [H1 H2]]. destruct e; simpl in *;
+        try congruence; try (destruct (nth_error _ a)); destruct a as [|[|[]]];
+        congruence || (apply IHp; eexists; intuition; eassumption).
+    - destruct e; simpl in *;
+        try congruence; try (destruct (nth_error _ a));
+        destruct a as [|[|[]]]; congruence || apply IHp; assumption.
   Qed.
 
   Lemma IsPath_chunk : forall e p c,
